leetcode/0069-sqrt.dfy
@@ -5,21 +5,21 @@ predicate sqrt(x: int, r: int) {
 }
 
 lemma uniqueSqrt(x: int, r1: int, r2: int)
-requires x >= 0 && r1 >= 0 && r2 >= 0;
+requires x >= 0 && r1 >= 0 && r2 >= 0
 ensures sqrt(x, r1) && sqrt(x, r2) ==> r1 == r2
 {}
 
 method mySqrt(x: int) returns (res: int)
-requires 0 <= x;
-ensures sqrt(x, res);
+requires 0 <= x
+ensures sqrt(x, res)
 {
     var l, r := 0, x;
     while (l <= r)
-    decreases r - l;
-    invariant l >= 0;
-    invariant r >= 0;
-    invariant l*l <= x;
-    invariant (r+1)*(r+1) > x;
+    decreases r - l
+    invariant l >= 0
+    invariant r >= 0
+    invariant l*l <= x
+    invariant (r+1)*(r+1) > x
     {
         var mid := (l + r) / 2;
         if (mid * mid <= x && (mid + 1) * (mid + 1) > x) {
