leetcode/1492-kthfactor.dfy
@@ -3,7 +3,7 @@ include "../lib/math/Factors.dfy"
 import opened FactorsModule
 
 method KthFactor(n: int, k: int) returns (r: int)
-  requires 0 < k <= n;
+  requires 0 < k <= n
   ensures r == -1 <==> k > |AllFactors(n)|
   ensures r > 0 <==> k <= |AllFactors(n)| && AllFactors(n)[k - 1] == r
 {
