lib/adt/BST.dfy
@@ -1,0 +1,20 @@
+include "BinaryTree.dfy"
+
+import opened BinaryTree
+
+predicate GEAll(x: int, xs: multiset<int>)
+{
+    forall v :: v in xs ==> x >= v
+}
+
+lemma GEAllEmpty(x: int, xs: multiset<int>)
+ensures |xs| == 0 ==> GEAll(x, xs)
+{
+}
+
+predicate BinarySearchTree?(t: Tree<int>)
+{
+    match t
+    case Nil => true
+    case Node(x, l, r) => GEAll(x, ToMS(l)) && GEAll(x, ToMS(r)) && BinarySearchTree?(l) && BinarySearchTree?(r)
+}
