lib/seq/Map.dfy
@@ -1,0 +1,26 @@
+function Cons<T>(x: T, xs: seq<T>) : seq<T> {
+    [x] + xs
+}
+
+function Map<A, B>(f: A -> B, xs: seq<A>): seq<B> {
+  if |xs| == 0 then [] else Cons(f(xs[0]), Map(f, xs[1..]))
+}
+
+// Functor laws: https://wiki.haskell.org/Functor
+// Functors must preserve identity morphisms
+lemma MapIdentity<T>(xs : seq<T>)
+ensures Map(x => x, xs) == xs
+{
+  if |xs| > 0 {
+    MapIdentity(xs[1..]);
+  }
+}
+
+// Functors preserve composition of morphisms
+lemma MapCompose<A, B, C>(xs: seq<A>, f: B -> C, g: A -> B)
+ensures Map(ys => f(g(ys)), xs) == Map(f, Map(g, xs))
+{
+  if |xs| > 0 {
+    MapCompose(xs[1..], f, g);
+  }
+}
